LeanSSZ.lean
@@ -11,3 +11,5 @@ import LeanSSZ.Core.Uint
 import LeanSSZ.Core.Bytes
 import LeanSSZ.Core.Vector
 import LeanSSZ.Core.Utils
+import LeanSSZ.Core.Sequence
+import LeanSSZ.Core.List
